Pauline/Tactic.lean
@@ -6,48 +6,6 @@ namespace Pauline.Tactic
 
 open Lean Lean.Expr Lean.Meta
 
-elab "sml_eval'" : tactic =>
-  Lean.Elab.Tactic.withMainContext do
-    let goal ← Lean.Elab.Tactic.getMainTarget
-    let expr_type ← Lean.Meta.inferType goal
-    dbg_trace f!"goal: {goal}\n\n{expr_type}"
-
-def myApply (goal : MVarId) (e : Expr) : MetaM (List MVarId) := do
-  -- Check that the goal is not yet assigned.
-  goal.checkNotAssigned `myApply
-  -- Operate in the local context of the goal.
-  goal.withContext do
-    -- Get the goal's target type.
-    let target ← goal.getType
-    -- Get the type of the given expression.
-    let type ← inferType e
-    -- If `type` has the form `∀ (x₁ : T₁) ... (xₙ : Tₙ), U`, introduce new
-    -- metavariables for the `xᵢ` and obtain the conclusion `U`. (If `type` does
-    -- not have this form, `args` is empty and `conclusion = type`.)
-    let (args, _, conclusion) ← forallMetaTelescopeReducing type
-    -- If the conclusion unifies with the target:
-    if ← isDefEq target conclusion then
-      -- Assign the goal to `e x₁ ... xₙ`, where the `xᵢ` are the fresh
-      -- metavariables in `args`.
-      goal.assign (mkAppN e args)
-      -- `isDefEq` may have assigned some of the `args`. Report the rest as new
-      -- goals.
-      let newGoals ← args.filterMapM λ mvar => do
-        let mvarId := mvar.mvarId!
-        if ! (← mvarId.isAssigned) && ! (← mvarId.isDelayedAssigned) then
-          return some mvarId
-        else
-          return none
-      return newGoals.toList
-    -- If the conclusion does not unify with the target, throw an error.
-    else
-      throwTacticEx `myApply goal m!"{e} is not applicable to goal with target {target}"
-
-elab "sml_step'" : tactic =>
-  Lean.Elab.Tactic.withMainContext do
-    sorry
-
-
 macro "sml_step_rfl" : tactic =>
   `(tactic| apply StepsExp.zero_step)
 
@@ -85,9 +43,10 @@ macro "sml_step_one" : tactic =>
    )
 
 macro "sml_step_tuple" : tactic =>
-  `(tactic| ( first | apply StepExp.tupleTlStep (by rewrite [isVal]; decide) (by simp)
+  `(tactic| ( first | apply StepExp.safeTupleTlStep
+                        (by rewrite [isVal]; decide) (by simp)
                       dbg_trace "step: tuple tl"
-                    | apply StepExp.tupleHdStep (by rewrite [isVal]; decide)
+                    | apply StepExp.safeTupleHdStep (by rewrite [isVal]; decide)
                       dbg_trace "step: tuple hd"
               -- try sml_step_one
             )
@@ -101,11 +60,21 @@ macro "sml_step_left_star" : tactic =>
             )
    )
 
+macro "sml_congr" : tactic =>
+  `(tactic| first | apply StepsExp.func_ext (by decide)
+                  | apply StepsExp.tuple_tl (by simp) (by simp)
+                  | apply StepsExp.tuple_hd (by simp)
+   )
+
 macro "sml_step" : tactic =>
   `(tactic| first | sml_step_rfl
+                  | sml_congr -- shld this be here?
                   | sml_step_left_star
                   | sml_step_tuple
                   | sml_step_one
    )
 
--- todo make SML tactic specific syntax category
+macro "sml_apply_ih" t:term : tactic =>
+  `(tactic| first | apply $t
+                  | apply StepsExp.split_int $t (by repeat sml_step)
+   )
